%% LyX 2.3.6.2 created this file.  For more info, see http://www.lyx.org/.
%% Do not edit unless you really know what you are doing.
\documentclass[english]{article}
\usepackage{mathptmx}
\usepackage[T1]{fontenc}
\usepackage[latin9]{inputenc}
\usepackage{amsmath}
\usepackage{babel}
\begin{document}
\textbf{Claim}. 

Write $P(p)\equiv\bar{p}(p)$ so I can type fast.

Suppose $P(p)$ is increasing from $P(0)=k\in(0,1)$ to $P(1)=1$.
Then on $(0,1)$:

\[
LHS(p)\equiv\frac{P(p)-p}{1-p}\textrm{ is decreasing in }p\textrm{ if }P(p)\textrm{ is strictly convex.}
\]
Proof.

$P(p)$ is convex on $(0,1)$ if and only if for all $0<p_{1}<p_{2}<1$
and $a\in(0,1)$,
\[
P(ap_{1}+(1-a)p_{2})<aP(p_{1})+(1-a)P(p_{2}).
\]

For arbitrary $p_{1}$ and $a\in(0,1)$, take $p_{2}=1$ and write
$p_{3}=ap_{1}+(1-a)$. 

Now write $q=aP(p_{1})+(1-a),$i.e., $q$ is the point on the line
segment between $P(p_{1})$ and 1. Then
\begin{align*}
 & \frac{q-p_{3}}{1-p_{3}}\\
= & \frac{aP(p_{1})+(1-a)-[ap_{1}+(1-a)]}{1-[ap_{1}+(1-a)]}\\
= & \frac{aP(p_{1})-ap_{1}}{a(1-p_{1})}\\
= & \frac{P(p_{1})-p_{1}}{1-p_{1}}.
\end{align*}
Last, observe that by convexity of $P$, 
\begin{align*}
P(p_{3}) & <aP(p_{1})+(1-a)P(p_{2})\\
 & =aP(p_{1})+(1-a)P(1)\\
 & =aP(p_{1})+(1-a)\\
 & =q.
\end{align*}

Putting these together
\[
\frac{P(p_{3})-p_{3}}{1-p_{3}}<\frac{P(p_{1})-p_{1}}{1-p_{1}}
\]
and because $p_{1}$ and $p_{3}>p_{1}$ were arbitrary we have proved
that $LHS(p)$ is decreasing.
\end{document}
